\documentclass[a4paper, 11pt]{article}

\usepackage{amsmath}
\usepackage{amssymb}
\usepackage{amsthm}
\usepackage{fullpage}

\newtheorem{theorem}{Theorem}
\newenvironment{pr}{\textbf{Proof.}}{\hfill\textbf{$\blacksquare$}}

\begin{document}

\begin{theorem}\label{theroem_label}
Let $I \subset \mathbb{R}$ be a nonempty open interval.
Then it holds for $f, g \in C^{\infty}(I)$ and $n \in \mathbb{N}$
\[(fg)^{(n)} = \sum_{k=0}^{n}\binom{n}{k}f^{(k)}g^{(n-k)}.\]
\end{theorem}
\noindent
\begin{pr}
    Proof by induction:

    For the base case is correct because 
    \[(fg)' = f'g + fg' = \binom{1}{1}f'g + \binom{1}{0}fg' = \sum_{k=0}^{1}\binom{1}{k}f^{(k)}g^{(1-k)}.\]

    For induction step assume that \eqref{theroem_label} holds for some $n \in \mathbb{N}$. That implies
    \begin{align*}
        (fg)^{(n+1)} &= \left((fg)^{(n)}\right)' \stackrel{\text{I.H.}}{=} \left(\sum_{k=0}^{n}\binom{n}{k}f^{(k)}g^{(n-k)}\right)'\\
        &= \sum_{k=0}^{n}\binom{n}{k}\left(f^{(k)}g^{(n-k)}\right)'\\
        &= \sum_{k=0}^{n}\binom{n}{k}\left(f^{(k+1)}g^{(n-k)}+f^{(k)}g^{(n-k+1)}\right)\\
        &= \sum_{k=0}^{n}\binom{n}{k}f^{(k+1)}g^{(n-k)} + \sum_{k=0}^{n}\binom{n}{k}f^{(k)}g^{(n-k+1)}\\
        &= \sum_{k=1}^{n+1}\binom{n}{k-1}f^{(k)}g^{(n-k+1)} + \sum_{k=0}^{n}\binom{n}{k}f^{(k)}g^{(n-k+1)}\\
        &= \sum_{k=1}^{n}\binom{n}{k-1}f^{(k)}g^{(n-k+1)} + \binom{n}{n}f^{(n+1)}g + \binom{n}{0}f g^{(n+1)}+ \sum_{k=1}^{n}\binom{n}{k}f^{(k)}g^{(n-k+1)}\\
        &= \left(\sum_{k=1}^{n}\left(\binom{n}{k-1} + \binom{n}{k}\right)f^{(k)}g^{(n-k+1)}\right) + \binom{n}{n}f^{(n+1)}g + \binom{n}{0}f g^{(n+1)}\\
        &= \left(\sum_{k=1}^{n}\binom{n+1}{k}f^{(k)}g^{(n-k+1)}\right) + \binom{n+1}{n+1}f^{(n+1)}g + \binom{n+1}{0}f g^{(n+1)}\\
        &= \sum_{k=0}^{n+1}\binom{n+1}{k}f^{(k)}g^{(n+1-k)}
    \end{align*}
\end{pr}

\end{document}